Verify receive, fix definitions to work with helping

new/proof/github_com/goose_lang/goose/model/channel/logatom/chan_au_base.v
@@ -8,51 +8,85 @@ From New.generatedproof.github_com.goose_lang.goose Require Import model.channel
 From New.proof.github_com.goose_lang Require Import primitive.
 From New.proof.github_com.goose_lang.std Require Import std_core.
 
-(* Inductive mathematical representation *)
+(** The mathematical model of channel states. This represents the logical
+    behavior of channels independent of the implementation details. *)
 Module chan_rep.
 Inductive t (V : Type) : Type :=
-| Buffered (buff : list V)
-| Idle
-| SndWait (v : V)
-| RcvWait  
-| SndDone (v : V)
-| RcvDone
-| Closed (draining : list V).
-  
-  (* Global Arguments for clean syntax *)
+| Buffered (buff: list V)     (* Buffered channel with pending messages *)
+| Idle                        (* Empty unbuffered channel, ready for operations *)
+| SndPending (v: V)          (* Unbuffered channel with sender waiting *)
+| RcvPending                 (* Unbuffered channel with receiver waiting *)
+| SndCommit (v: V)           (* Sender committed, waiting for receiver to complete *)
+| RcvCommit                  (* Receiver committed, waiting for sender to complete *)
+| Closed (draining: list V)  (* Closed channel, possibly draining remaining messages *)
+.
+
   Global Arguments Buffered {V}.
+  Global Arguments Idle {V}.
+  Global Arguments SndPending {V}.
+  Global Arguments RcvPending {V}.
+  Global Arguments SndCommit {V}.
+  Global Arguments RcvCommit {V}.
+  Global Arguments Closed {V}.
+
+End chan_rep.
+
+(** The state machine representation matching the model implementation.
+    This is slightly different from the mathematical representation
+    in that we don't go to the SndWait state logically until an offer 
+    is about to be accepted. *)
+Inductive chan_phys_state (V : Type) : Type :=
+| Buffered (buff: list V)     (* Channel with buffered messages *)
+| Idle                        (* Ready for operations *)
+| SndWait (v : V)            (* Sender offers *)
+| RcvWait                    (* Receiver offers *)
+| SndDone (v : V)            (* Sender operation completed, handshake in progress *)
+| RcvDone (v : V)            (* Receiver operation completed, handshake in progress *)
+| Closed (draining: list V)  (* Closed channel *)
+.
+
   Global Arguments Idle {V}.
   Global Arguments SndWait {V}.
   Global Arguments RcvWait {V}.
   Global Arguments SndDone {V}.
   Global Arguments RcvDone {V}.
-  Global Arguments Buffered {V}.
   Global Arguments Closed {V}.
+  Global Arguments Buffered {V}.
 
-  Definition buffer_valid {V} (c : chan_rep.t V) (cap: w64) : Prop :=
-  match c with
-  | chan_rep.Buffered buff =>
-    length buff ≤ uint.Z cap
-  | chan_rep.Closed draining =>
-    length draining ≤ uint.Z cap
-  | _ => True (* Invariant is vacuously true for unbuffered or empty closed states *)
-  end.
+(** The offer protocol coordinates handshakes between senders and receivers
+    in unbuffered channels. An "offer" represents a pending operation that
+    can be accepted by the other party. This ghost state ensures that 
+    an outstanding offer can only be accepted or left as-is for when we lock
+    the channel to check the status. *)
+Inductive offer_lock (V : Type) : Type :=
+| Snd (v : V)                (* Sender has made an offer *)
+| Rcv                        (* Receiver has made an offer *)
+.
 
-End chan_rep.
+  Global Arguments Snd {V}.
+  Global Arguments Rcv {V}.
 
-(* Ghost state management *)
+(** Ghost names for tracking various aspects of channel state in the logic *)
 Record chan_names := {
-  offer_name : gname;   (* For unbuffered offer/accept protocol *)
-  state_name : gname;   (* For the main channel state *)
+  state_name : gname;                    (* Main channel state *)
+  offer_lock_name : gname;               (* Offer protocol lock *)
+  offer_parked_prop_name : gname;        (* The saved prop that we can leave with the channel to support select *)
+  offer_parked_pred_name : gname;        (* The saved continuation for receive, which is a predicate on v, ok *)
+  offer_continuation_name : gname;       (* The continuation for send *)
 }.
 
+(** Type class for ghost state associated with channels *)
 Class chanGhostStateG Σ V := ChanGhostStateG {
-  offer_tokG :: ghost_varG Σ (option V);
-  chan_repG :: ghost_varG Σ (chan_rep.t V);
+  offerG :: ghost_varG Σ (chan_rep.t V);
+  offer_lockG :: ghost_varG Σ (option (offer_lock V));
+  offer_parked_propG :: savedPropG Σ;
+  offer_parked_predG :: savedPredG Σ (V * bool);
+  continuation_parkedG :: savedPropG Σ;
 }.
 
 Definition chanGhostStateΣ V : gFunctors :=
-  #[ ghost_varΣ (option V); ghost_varΣ (chan_rep.t V) ].
+  #[ ghost_varΣ (chan_rep.t V); ghost_varΣ (option (offer_lock V));
+     savedPropΣ; savedPredΣ  (V * bool) ].
 
 #[global] Instance subG_chanGhostStateG Σ V :
   subG (chanGhostStateΣ V) Σ → chanGhostStateG Σ V.
@@ -63,124 +97,265 @@ Context `{hG: heapGS Σ, !ffi_semantics _ _}.
 Context `{!chanGhostStateG Σ V}.
 Context `{!IntoVal V}.
 Context `{!IntoValTyped V t}.
-  
-(* Offer tokens for unbuffered channels *)
-Definition idle_tok (γ : gname) : iProp Σ :=
-    ghost_var γ 1%Qp None.
-  
-(* Send offer is outgoing, we can unlock the channel and know that the channel was
-  untouched other then by a receiver accepting the offer *)
-Definition snd_wait_tok (γ : gname) (v: V) : iProp Σ :=
-    ghost_var γ (1/2%Qp) (Some v).
 
-(* Almost symmetric to snd_wait_tok, but we don't need to encode a value *)
-Definition rcv_wait_tok (γ : gname) : iProp Σ :=
-    ghost_var γ (1/2%Qp) None.
-
-Lemma idle_to_two_snd_wait γ v :
-  idle_tok γ ==∗ snd_wait_tok γ v ∗ snd_wait_tok γ v.
+(* Remove the later from a saved prop if we have later credits. *)
+Lemma saved_prop_lc_agree γ dq1 dq2 P Q :
+   £ 1 -∗ saved_prop_own γ dq1 P -∗ saved_prop_own γ dq2 Q -∗ |={⊤}=> (P ≡ Q).
 Proof.
-  iIntros "Hidle".
-  iMod (ghost_var_update (Some v) γ _ with "Hidle") as "Hfull".
-  iDestruct "Hfull" as "[Hs1 Hs2]".
-  iModIntro. iFrame.
+  iIntros "Hlc HP HQ".
+  iDestruct (saved_prop_agree with "HP HQ") as "Heq".
+  iMod (lc_fupd_elim_later with "Hlc Heq") as "H3".
+  iModIntro. done.
 Qed.
 
-Lemma idle_to_two_rcv_wait γ :
-  idle_tok γ ==∗ rcv_wait_tok γ ∗ rcv_wait_tok γ.
-Proof.
-  iIntros "Hidle".
-  iMod (ghost_var_update _ γ _ with "Hidle") as "Hfull".
-  iDestruct "Hfull" as "[Hs1 Hs2]".
-  iModIntro. iFrame.
-Qed.
-
-Lemma two_snd_wait_to_idle γ v1 v2 :
-  snd_wait_tok γ v1 -∗ snd_wait_tok γ v2 ==∗ idle_tok γ.
-Proof.
-  iIntros "Hs1 Hs2".
-  iCombine "Hs1" "Hs2" as "Hfull".
-  iMod (ghost_var_update None γ _ with "Hfull") as "Hidle".
-  iModIntro. iExact "Hidle".
-Qed.
-
-Lemma two_rcv_wait_to_idle γ :
-  rcv_wait_tok γ -∗ rcv_wait_tok γ ==∗ idle_tok γ.
-Proof.
-  iIntros "Hs1 Hs2".
-  iCombine "Hs1" "Hs2" as "Hfull".
-  iMod (ghost_var_update None γ _ with "Hfull") as "Hidle".
-  iModIntro. iExact "Hidle".
-Qed.
-
-
-Definition offer_auth (γ : chan_names) (s : chan_rep.t V) : iProp Σ :=
+(** Maps physical channel states to their heap representations.
+    Each state corresponds to specific field values in the Go struct. *)
+Definition chan_phys (ch: loc) (s: chan_phys_state V) : iProp Σ :=
   match s with
-  | chan_rep.SndWait v   => snd_wait_tok γ.(offer_name) v
-  | chan_rep.RcvWait     => rcv_wait_tok γ.(offer_name)
-  | chan_rep.SndDone v   => rcv_wait_tok γ.(offer_name)
-  | chan_rep.RcvDone     =>  ∃ v, snd_wait_tok γ.(offer_name) v
-  | _  => idle_tok γ.(offer_name)
-  end.
+    | Closed [] =>
+        ∃ (slice_val: slice.t),
+        "state" ∷ ch ↦s[(channel.Channel.ty t) :: "state"] (W64 6) ∗
+        "slice" ∷ own_slice slice_val (DfracOwn 1) ([] : list V) ∗
+        "slice_cap" ∷ own_slice_cap V slice_val (DfracOwn 1) ∗
+        "buffer" ∷ ch ↦s[(channel.Channel.ty t) :: "buffer"] slice_val
+    | Closed draining =>
+        ∃ (slice_val: slice.t),
+        "state" ∷ ch ↦s[(channel.Channel.ty t) :: "state"] (W64 6) ∗
+        "slice" ∷ own_slice slice_val (DfracOwn 1) draining ∗
+        "slice_cap" ∷ own_slice_cap V slice_val (DfracOwn 1) ∗
+        "buffer" ∷ ch ↦s[(channel.Channel.ty t) :: "buffer"] slice_val
+    | Buffered buff =>
+        ∃ (slice_val: slice.t),
+        "state" ∷ ch ↦s[(channel.Channel.ty t) :: "state"] (W64 0) ∗
+        "slice" ∷ own_slice slice_val (DfracOwn 1) buff ∗
+        "slice_cap" ∷ own_slice_cap V slice_val (DfracOwn 1) ∗
+        "buffer" ∷ ch ↦s[(channel.Channel.ty t) :: "buffer"] slice_val
+    | Idle =>
+        ∃ (v:V) (slice_val: slice.t),
+        "state" ∷ ch ↦s[(channel.Channel.ty t) :: "state"] (W64 1) ∗
+        "v" ∷ ch ↦s[(channel.Channel.ty t) :: "v"] v ∗ 
+        "slice" ∷ own_slice slice_val (DfracOwn 1) ([] : list V) ∗
+        "slice_cap" ∷ own_slice_cap V slice_val (DfracOwn 1) ∗ 
+        "buffer" ∷ ch ↦s[(channel.Channel.ty t) :: "buffer"] slice_val
+    | SndWait v =>
+        ∃ (slice_val: slice.t),
+        "state" ∷ ch ↦s[(channel.Channel.ty t) :: "state"] (W64 2) ∗
+        "v" ∷ ch ↦s[(channel.Channel.ty t) :: "v"] v ∗  
+        "slice" ∷ own_slice slice_val (DfracOwn 1) ([] : list V) ∗
+        "slice_cap" ∷ own_slice_cap V slice_val (DfracOwn 1) ∗ 
+        "buffer" ∷ ch ↦s[(channel.Channel.ty t) :: "buffer"] slice_val
+    | RcvWait =>
+        ∃ (v:V) (slice_val: slice.t),
+        "state" ∷ ch ↦s[(channel.Channel.ty t) :: "state"] (W64 3) ∗
+        "v" ∷ ch ↦s[(channel.Channel.ty t) :: "v"] v ∗ 
+        "slice" ∷ own_slice slice_val (DfracOwn 1) ([] : list V) ∗
+        "slice_cap" ∷ own_slice_cap V slice_val (DfracOwn 1) ∗ 
+        "buffer" ∷ ch ↦s[(channel.Channel.ty t) :: "buffer"] slice_val
+    | SndDone v =>
+        ∃ (slice_val: slice.t),
+        "state" ∷ ch ↦s[(channel.Channel.ty t) :: "state"] (W64 4) ∗
+        "v" ∷ ch ↦s[(channel.Channel.ty t) :: "v"] v ∗  
+        "slice" ∷ own_slice slice_val (DfracOwn 1) ([] : list V) ∗
+        "slice_cap" ∷ own_slice_cap V slice_val (DfracOwn 1) ∗ 
+        "buffer" ∷ ch ↦s[(channel.Channel.ty t) :: "buffer"] slice_val
+    | RcvDone v =>
+        ∃ (slice_val: slice.t),
+        "state" ∷ ch ↦s[(channel.Channel.ty t) :: "state"] (W64 5) ∗ 
+        "v" ∷ ch ↦s[(channel.Channel.ty t) :: "v"] v ∗ 
+        "slice" ∷ own_slice slice_val (DfracOwn 1) ([] : list V) ∗
+        "slice_cap" ∷ own_slice_cap V slice_val (DfracOwn 1) ∗ 
+        "buffer" ∷ ch ↦s[(channel.Channel.ty t) :: "buffer"] slice_val
+    end.
 
-Lemma offer_snd_coherent γ (s : chan_rep.t V) v :
-  offer_auth γ s -∗ snd_wait_tok γ.(offer_name) v -∗
-  ⌜s = chan_rep.SndWait v ∨ s = chan_rep.RcvDone ⌝.
+(** Bundles together offer-related ghost state for atomic operations *)
+Definition saved_offer (γ : chan_names) (q : Qp)
+  (lock_val : option (offer_lock V))
+  (parked_prop continuation_prop : iProp Σ) : iProp Σ :=
+  ghost_var γ.(offer_lock_name) q lock_val ∗
+  saved_prop_own γ.(offer_parked_prop_name) (DfracOwn q) parked_prop ∗
+  saved_prop_own γ.(offer_continuation_name) (DfracOwn q) continuation_prop.
+
+Notation offer_bundle_full γ := (saved_offer γ 1%Qp).
+Notation offer_bundle_half γ := (saved_offer γ (1/2)%Qp).
+
+Definition offer_bundle_empty (γ : chan_names) : iProp Σ :=
+  offer_bundle_full γ None True True.
+
+Lemma offer_idle_to_send γ v parked_prop cont :
+  offer_bundle_empty γ ==∗
+  offer_bundle_half γ (Some (Snd v)) parked_prop cont ∗
+  offer_bundle_half γ (Some (Snd v)) parked_prop cont.
 Proof.
-  iIntros "Hpiece Htok".
-  destruct s; simpl.
-  - 
-     iDestruct (ghost_var_valid_2 with "[$Hpiece] [$Htok]") as "%Hinvalid".
-     destruct Hinvalid as [Hbad _]. apply  (Qp.not_add_le_r 1 (1/2)) in Hbad. contradiction.
-  - 
-     iDestruct (ghost_var_valid_2 with "[$Hpiece] [$Htok]") as "%Hinvalid".
-     destruct Hinvalid as [Hbad _]. apply  (Qp.not_add_le_r 1 (1/2)) in Hbad. contradiction.
-  - iDestruct (ghost_var_agree with "Hpiece Htok") as %Heq. inversion Heq. subst. iPureIntro. left. reflexivity.
-  - iDestruct (ghost_var_agree with "Hpiece Htok") as %Eq.  
-iPureIntro.
-exfalso. discriminate Eq. 
-  -  iDestruct (ghost_var_agree with "Hpiece Htok") as %Eq. 
-iPureIntro.
-exfalso. discriminate Eq.
-  - iPureIntro. right. done.
-  - iDestruct (ghost_var_valid_2 with "[$Hpiece] [$Htok]") as "%Hinvalid".
-    destruct Hinvalid as [Hbad _]. apply  (Qp.not_add_le_r 1 (1/2)) in Hbad. contradiction.
+  iIntros "[Hlock [Hoffer Hcont]]".
+  iMod (ghost_var_update (Some (Snd v)) with "Hlock") as "[Hlock1 Hlock2]".
+  iMod (saved_prop_update cont with "Hcont") as "[Hcont1 Hcont2]".
+  iMod (saved_prop_update parked_prop with "Hoffer") as "[Hoffer1 Hoffer2]".
+  iModIntro. iFrame.
 Qed.
 
-Lemma offer_rcv_coherent γ (s : chan_rep.t V) :
-  offer_auth γ s -∗ rcv_wait_tok γ.(offer_name) -∗
-  ⌜s = chan_rep.RcvWait ∨ ∃ v, s = chan_rep.SndDone v⌝.
+Lemma offer_send_to_idle γ v parked_prop cont :
+  offer_bundle_half γ (Some (Snd v)) parked_prop cont -∗
+   offer_bundle_half γ (Some (Snd v)) parked_prop cont ==∗
+  offer_bundle_empty γ.
 Proof.
-  iIntros "Hpiece Htok".
-  destruct s; simpl in *.
-  - iDestruct (ghost_var_valid_2 with "Hpiece Htok") as %[Hle _].
-    iPureIntro. exfalso. exact (Qp.not_add_le_l 1 (1/2)%Qp Hle).
-  - iDestruct (ghost_var_valid_2 with "Hpiece Htok") as %[Hle _]. 
-    iPureIntro. exfalso. exact (Qp.not_add_le_l 1 (1/2)%Qp Hle).
-  - iDestruct (ghost_var_agree with "Hpiece Htok") as %Eq. iPureIntro. exfalso. discriminate Eq.
-  - iPureIntro. left; reflexivity.
-  - iPureIntro. right. exists v. done.
-  - iNamed "Hpiece".
-    iDestruct (ghost_var_agree with "Hpiece Htok") as %Eq. iPureIntro. exfalso. discriminate Eq.
-  - iDestruct (ghost_var_valid_2 with "Hpiece Htok") as %[Hle _]. 
-    iPureIntro. exfalso. exact (Qp.not_add_le_l 1 (1/2)%Qp Hle).
+  iIntros "[Hlock [Hoffer Hcont]]".
+  iIntros "[Hlock2 [Hoffer2 Hcont2]]".
+  iCombine "Hlock Hlock2" as "Hlock".
+  iMod (saved_prop_update_halves True with "Hoffer Hoffer2") as "[Hoffer Hoffer2]".
+  iMod (saved_prop_update_halves True with "Hcont Hcont2") as "[Hcont Hcont2]".
+  iCombine "Hcont Hcont2" as "Hcont".
+  iCombine "Hoffer Hoffer2" as "Hoffer".
+  iMod (ghost_var_update None with "Hlock") as "Hlock".
+  iModIntro. unfold offer_bundle_empty. unfold offer_bundle_full. iFrame.
+  unfold saved_prop_own.
+  rewrite dfrac_op_own.
+  rewrite Qp.half_half.
+  iFrame.
 Qed.
 
+Lemma offer_idle_to_recv γ parked_prop cont:
+  offer_bundle_empty γ ==∗
+  offer_bundle_half γ (Some Rcv) parked_prop cont ∗
+  offer_bundle_half γ (Some Rcv) parked_prop cont.
+Proof.
+   iIntros "[Hlock [Hoffer Hcont]]".
+  iMod (ghost_var_update (Some (Rcv)) with "Hlock") as "[Hlock1 Hlock2]".
+  iMod (saved_prop_update cont with "Hcont") as "[Hcont1 Hcont2]".
+  iMod (saved_prop_update parked_prop with "Hoffer") as "[Hoffer1 Hoffer2]".
+  iModIntro. iFrame.
+Qed.
 
-(* ghost state for channel mathematical representation. *)
+Lemma offer_recv_to_idle γ parked_prop cont :
+  offer_bundle_half γ (Some Rcv) parked_prop cont -∗
+   offer_bundle_half γ (Some Rcv) parked_prop cont ==∗
+  offer_bundle_empty γ.
+Proof.
+  iIntros "[Hlock [Hoffer Hcont]]".
+  iIntros "[Hlock2 [Hoffer2 Hcont2]]".
+  iCombine "Hlock Hlock2" as "Hlock".
+  iMod (saved_prop_update_halves True with "Hoffer Hoffer2") as "[Hoffer Hoffer2]".
+  iMod (saved_prop_update_halves True with "Hcont Hcont2") as "[Hcont Hcont2]".
+  iCombine "Hcont Hcont2" as "Hcont".
+  iCombine "Hoffer Hoffer2" as "Hoffer".
+  iMod (ghost_var_update None with "Hlock") as "Hlock".
+  iModIntro. unfold offer_bundle_empty. unfold offer_bundle_full. iFrame.
+  unfold saved_prop_own.
+  rewrite dfrac_op_own.
+  rewrite Qp.half_half.
+  iFrame.
+Qed.
+
+Lemma offer_reset γ :
+  ∀ parked_prop cont state,
+   offer_bundle_full γ state parked_prop cont ==∗
+  offer_bundle_empty γ.
+Proof.
+  intros parked_prop cont state.
+  iIntros "[Hlock [Hoffer Hcont]]".
+  iMod (ghost_var_update None with "Hlock") as "Hlock".
+  iMod (saved_prop_update True with "Hcont") as "Hcont".
+  iMod (saved_prop_update True with "Hoffer") as "Hoffer".
+  iModIntro.
+  iFrame.
+Qed.
+
+Lemma offer_bundle_agree γ q1 q2
+  lock1 parked1 cont1 lock2 parked2 cont2 :
+  saved_offer γ q1 lock1 parked1 cont1 ∗
+  saved_offer γ q2 lock2 parked2 cont2 ⊢
+  ⌜lock1 = lock2⌝ ∗
+  ▷(parked1 ≡ parked2) ∗ ▷(cont1 ≡ cont2).
+Proof.
+  iIntros "[[Hl1 [Hp1 Hc1]] [Hl2 [Hp2 Hc2]]]".
+  iDestruct (ghost_var_agree with "Hl1 Hl2") as %->.
+  iDestruct (saved_prop_agree with "Hp1 Hp2") as "Hp_eq".
+  iDestruct (saved_prop_agree with "Hc1 Hc2") as "Hc_eq".
+  auto.
+Qed.
+
+Lemma offer_bundle_lc_agree γ
+  lock1 parked1 cont1 lock2 parked2 cont2 :
+  £ 1 -∗ £ 1 -∗
+  saved_offer γ (1/2) lock1 parked1 cont1 -∗
+  saved_offer γ (1/2) lock2 parked2 cont2 -∗
+  |={⊤}=> ⌜lock1 = lock2⌝ ∗
+         (parked1 ≡ parked2) ∗ (cont1 ≡ cont2) ∗
+         offer_bundle_empty γ.
+Proof.
+  iIntros "Hlc1".
+  iIntros "Hlc2".
+  iIntros "[Hl1 [Hp1 Hc1]]".
+  iIntros "[Hl2 [Hp2 Hc2]]".
+   iDestruct (ghost_var_agree with "[$Hl1] [$Hl2]") as %->.
+  iDestruct (saved_prop_agree with "[$Hp1] [$Hp2]") as "#Hp_eq".
+  iDestruct (saved_prop_agree with "[$Hc1] [$Hc2]") as "#Hc_eq".
+
+  iMod (lc_fupd_elim_later with "Hlc1 Hp_eq") as "Hp_eq1".
+  iMod (lc_fupd_elim_later with "Hlc2 Hc_eq") as "Hc_eq1".
+  unfold offer_bundle_empty. unfold offer_bundle_full.
+  iFrame.
+  iSplitR; first done.  (* ⌜lock2 = lock2⌝ is trivial *)
+
+(* Combine and update ghost variable *)
+iCombine "Hl1 Hl2" as "Hlock".
+iMod ((ghost_var_update None) with "Hlock") as "Hlock".
+
+(* Update saved propositions using halves lemmas *)
+iMod (saved_prop_update_halves True with "Hp1 Hp2") as "[Hp1 Hp2]".
+iMod (saved_prop_update_halves True with "Hc1 Hc2") as "[Hc1 Hc2]".
+
+(* Combine the updated halves to get full ownership *)
+iCombine "Hp1 Hp2" as "Hparked".
+iCombine "Hc1 Hc2" as "Hcont".
+
+(* Simplify the combined fractions *)
+rewrite dfrac_op_own Qp.half_half.
+
+iFrame.
+  auto.
+Qed.
+
+Lemma saved_offer_fractional_invalid γ q1 q2 lock1 parked1 cont1 lock2 parked2 cont2 :
+  (1 < q1 + q2)%Qp →
+  saved_offer γ q1 lock1 parked1 cont1 -∗
+  saved_offer γ q2 lock2 parked2 cont2 -∗
+  False.
+Proof.
+  iIntros (Hq) "[Hlock1 [Hp1 Hc1]] [Hlock2 [Hp2 Hc2]]".
+  iDestruct (ghost_var_valid_2 with "Hlock1 Hlock2") as "[%Hvalid _]".
+  iPureIntro.
+apply Qp.lt_nge in Hq.
+contradiction.
+Qed.
+
+Lemma saved_offer_half_full_invalid γ lock1 parked1 cont1 lock2 parked2 cont2 :
+  saved_offer γ (1/2) lock1 parked1 cont1 -∗
+  saved_offer γ 1 lock2 parked2 cont2 -∗
+  False.
+Proof.
+  iApply saved_offer_fractional_invalid.
+  compute_done. (* 1/2 + 1 = 3/2 > 1 *)
+Qed.
+
 Definition chan_rep (γ : gname) (q : Qp) (s : chan_rep.t V) : iProp Σ :=
   ghost_var γ q s.
+
 Notation chan_rep_full γ s := (chan_rep γ 1 s).
 Notation chan_rep_half γ s := (chan_rep γ (1/2)%Qp s).
 Notation chan_rep_auth γ s := (chan_rep_half γ s).
 Notation chan_rep_frag γ s := (chan_rep_half γ s).
+
 Lemma chan_rep_update γ s s' :
   chan_rep_full γ s ==∗ chan_rep_full γ s'.
 Proof.
-  iApply (ghost_var_update s' γ s). Qed.
+  iApply (ghost_var_update s' γ s). 
+Qed.
+
 Lemma chan_rep_agree γ q1 q2 s s' :
   chan_rep γ q1 s -∗ chan_rep γ q2 s' -∗ ⌜s = s'⌝.
-Proof. iIntros "H1 H2". by iApply (ghost_var_agree with "H1 H2"). Qed.
+Proof. 
+  iIntros "H1 H2". by iApply (ghost_var_agree with "H1 H2"). 
+Qed.
 
 Lemma chan_rep_combine γ s s' :
   chan_rep_half γ s -∗ chan_rep_half γ s' -∗ ⌜s = s'⌝ -∗ chan_rep_full γ s.
@@ -188,127 +363,234 @@ Proof.
   iIntros "H1 H2 %H3". iDestruct (chan_rep_agree with "H1 H2") as %->.
   iCombine "H1" "H2" as "H". done.
 Qed.
+
 Lemma chan_rep_halves_update γ s1 s2 s' :
   chan_rep_half γ s1 -∗ chan_rep_half γ s2 ==∗
      chan_rep_half γ s' ∗ chan_rep_half γ s'.
 Proof.
 Admitted.
 
-
-(* Physical state helper utility for the channel model that uses a simple blocking
-   queue for buffered channels and an offer state machine for unbuffered channels
-*)
-
-  (* Unified physical state predicate *)
-  Definition chan_phys (ch: loc) (s: chan_rep.t V) 
-       : iProp Σ :=
-    match s with
-    | chan_rep.Closed [] => 
-        ∃ (slice_val: slice.t),
-        "state" ∷ ch ↦s[(channel.Channel.ty t) :: "state"] (W64 6) ∗ 
-        "slice" ∷ own_slice slice_val (DfracOwn 1) ([] : list V) ∗
-        "slice_cap" ∷ own_slice_cap V slice_val (DfracOwn 1) ∗ 
-        "buffer" ∷ ch ↦s[(channel.Channel.ty t) :: "buffer"] slice_val
-    | chan_rep.Closed draining =>
-        ∃ (slice_val: slice.t),
-        "state" ∷ ch ↦s[(channel.Channel.ty t) :: "state"] (W64 6) ∗
-        "slice" ∷ own_slice slice_val (DfracOwn 1) draining ∗
-        "slice_cap" ∷ own_slice_cap V slice_val (DfracOwn 1) ∗ 
-        "buffer" ∷ ch ↦s[(channel.Channel.ty t) :: "buffer"] slice_val
-    | chan_rep.Buffered buff => 
-        ∃ (slice_val: slice.t),
-        "state" ∷ ch ↦s[(channel.Channel.ty t) :: "state"] (W64 0) ∗
-        "slice" ∷ own_slice slice_val (DfracOwn 1) buff ∗
-        "slice_cap" ∷ own_slice_cap V slice_val (DfracOwn 1) ∗ 
-        "buffer" ∷ ch ↦s[(channel.Channel.ty t) :: "buffer"] slice_val
-    | chan_rep.Idle => 
-      ∃ (v:V) (slice_val: slice.t),
-      "state" ∷ ch ↦s[(channel.Channel.ty t) :: "state"] (W64 1) ∗
-      "v" ∷ ch ↦s[(channel.Channel.ty t) :: "v"] v ∗ 
-        "slice" ∷ own_slice slice_val (DfracOwn 1) ([] : list V) ∗
-        "slice_cap" ∷ own_slice_cap V slice_val (DfracOwn 1) ∗ 
-        "buffer" ∷ ch ↦s[(channel.Channel.ty t) :: "buffer"] slice_val
-    | chan_rep.SndWait v => 
-      ∃ (slice_val: slice.t),
-      "state" ∷ ch ↦s[(channel.Channel.ty t) :: "state"] (W64 2) ∗
-      "v" ∷ ch ↦s[(channel.Channel.ty t) :: "v"] v ∗  
-        "slice" ∷ own_slice slice_val (DfracOwn 1) ([] : list V) ∗
-        "slice_cap" ∷ own_slice_cap V slice_val (DfracOwn 1) ∗ 
-        "buffer" ∷ ch ↦s[(channel.Channel.ty t) :: "buffer"] slice_val
-    | chan_rep.RcvWait => 
-      ∃ (v:V) (slice_val: slice.t),
-      "state" ∷ ch ↦s[(channel.Channel.ty t) :: "state"] (W64 3) ∗
-      "v" ∷ ch ↦s[(channel.Channel.ty t) :: "v"] v ∗ 
-        "slice" ∷ own_slice slice_val (DfracOwn 1) ([] : list V) ∗
-        "slice_cap" ∷ own_slice_cap V slice_val (DfracOwn 1) ∗ 
-        "buffer" ∷ ch ↦s[(channel.Channel.ty t) :: "buffer"] slice_val
-    | chan_rep.SndDone v => 
-      ∃ (slice_val: slice.t),
-      "state" ∷ ch ↦s[(channel.Channel.ty t) :: "state"] (W64 4) ∗
-      "v" ∷ ch ↦s[(channel.Channel.ty t) :: "v"] v ∗  
-        "slice" ∷ own_slice slice_val (DfracOwn 1) ([] : list V) ∗
-        "slice_cap" ∷ own_slice_cap V slice_val (DfracOwn 1) ∗ 
-        "buffer" ∷ ch ↦s[(channel.Channel.ty t) :: "buffer"] slice_val
-    | chan_rep.RcvDone => 
-      ∃ (v:V) (slice_val: slice.t),
-      "state" ∷ ch ↦s[(channel.Channel.ty t) :: "state"] (W64 5) ∗ 
-      "v" ∷ ch ↦s[(channel.Channel.ty t) :: "v"] v ∗ 
-        "slice" ∷ own_slice slice_val (DfracOwn 1) ([] : list V) ∗
-        "slice_cap" ∷ own_slice_cap V slice_val (DfracOwn 1) ∗ 
-        "buffer" ∷ ch ↦s[(channel.Channel.ty t) :: "buffer"] slice_val
-    end.
-
-(* TODO: Add select physical state *)
-
-(* Ownership *)
-
-Definition cap_rel (cap : w64) (s : chan_rep.t V) : Prop :=
+Definition chan_cap_valid (s : chan_rep.t V) (cap: Z) : Prop :=
   match s with
-  (* Once we're closed and drained, unbuffered/buffered work the same *)
-  | chan_rep.Closed []                      => True
-  | chan_rep.Buffered _ | chan_rep.Closed _ => cap ≠ W64 0 ∧ sint.Z cap > 0
-  | _                                       => cap = W64 0
+  | chan_rep.Buffered _ => (0 < cap)%Z     
+  | chan_rep.Closed [] => True              (* Empty closed channels might have been unbuffered, doesn't matter *)
+  | chan_rep.Closed _ => (0 < cap)%Z (* Draining closed channels are buffered channels *)
+  | _ => cap = 0                            (* All other states are unbuffered *)
   end.
-  
-  (* What goes inside the mutex invariant *)
-  Definition chan_inv_inner (ch: loc) (cap:w64) (γ: chan_names) : iProp Σ :=
-    ∃ (s : chan_rep.t V),
-      "phys" ∷ chan_phys ch s ∗
-      "auth" ∷ chan_rep_auth γ.(state_name) s ∗
-      "%Hcap"  ∷  
-        ⌜cap_rel cap s⌝
-      ∗  
-      (* Offer ghost state for unbuffered channels *)
-      "offer"  ∷ offer_auth γ s.
-      
-  (* Public channel interface - what clients see *)
-  Definition is_channel (ch: loc) (cap :w64) (γ: chan_names) : iProp Σ :=
-    ∃ (mu_loc: loc) (s: chan_rep.t V),
-      "#cap" ∷ ch ↦s[(channel.Channel.ty t) :: "cap"]□ cap ∗
-      "#mu" ∷ ch ↦s[(channel.Channel.ty t) :: "lock"]□ mu_loc ∗
-      "#lock" ∷ is_Mutex mu_loc (chan_inv_inner ch cap γ).
-      
-  (* Fractional ownership for protocol development *)
-  Definition own_channel (ch: loc) (s: chan_rep.t V) (cap: w64) (γ: chan_names) : iProp Σ :=
-     "Hchanrepfrag" ∷ chan_rep_frag γ.(state_name) s ∗ "%Hbuffvalid" ∷ ⌜ chan_rep.buffer_valid s cap ⌝.
 
-(* Helper lemmas *)
-  
-  (* Persistence *)
-  Global Instance is_channel_pers ch cap γ : Persistent (is_channel ch cap γ).
-  Proof.
-  Admitted.
-  
-  (* Timelessness *)
-  Global Instance own_channel_timeless ch s cap γ : Timeless (own_channel ch s cap γ).
-  Proof.
+(** ** Channel Ownership Predicate *)
+
+(** Represents ownership of a channel with its logical state *)
+Definition own_channel (ch: loc) (cap: Z) (s: chan_rep.t V) (γ: chan_names) : iProp Σ :=
+  "Hchanrepfrag" ∷ chan_rep_half γ.(state_name) s ∗
+  "%Hcapvalid" ∷ ⌜chan_cap_valid s cap⌝.
+
+Lemma own_channel_agree ch cap cap' s s' γ :
+   own_channel ch cap s γ -∗ own_channel ch cap' s' γ -∗ ⌜s = s'⌝.
+Proof. 
+  iIntros "H1 H2". iNamed "H1". iDestruct "H2" as "[Hoc %Hcap]".
+  iDestruct (ghost_var_agree with "[$Hchanrepfrag] [$Hoc]") as "%Hag".
+  unfold chan_cap_valid in *.
+  by iApply (ghost_var_agree with "Hchanrepfrag Hoc"). 
+Qed.
+
+Lemma own_channel_halves_update ch cap s s' s'' γ :
+  own_channel ch cap s γ -∗ own_channel ch cap s' γ ==∗
+  own_channel ch cap s'' γ ∗ own_channel ch cap s'' γ.
+Proof.
   Admitted.
 
-  Lemma is_channel_not_null ch γ cap :
-    is_channel ch γ cap -∗ ⌜ch ≠ null⌝.
-  Proof.
-  Admitted.
+(** Type alias for convenience: converts postcondition to predicate format *)
+Definition K (Φ : V → bool → iProp Σ) : (V * bool) → iProp Σ :=
+  λ '(v,b), Φ v b.
+
+(** Inner atomic update for receive completion (second phase of handshake) *)
+Definition rcv_au_inner ch (cap: Z) (γ: chan_names) (Φ : V → bool → iProp Σ) : iProp Σ :=
+   |={⊤,∅}=>
+    ▷∃ s, "Hocinner" ∷ own_channel ch cap s γ ∗
+     "Hcontinner" ∷
+    (match s with
+    (* Case: Sender has committed, complete the exchange *)
+    | chan_rep.SndCommit v => own_channel ch cap chan_rep.Idle γ ={∅,⊤}=∗ Φ v true
+    (* Case: Channel is closed with no messages *)
+    | chan_rep.Closed [] => own_channel ch cap s γ ={∅,⊤}=∗ Φ (default_val V) false
+    | _ => True
+    end).
+
+(** Slow path receive: may need to block and wait *)
+Definition rcv_au_slow ch (cap: Z) (γ: chan_names) (Φ : V → bool → iProp Σ) : iProp Σ :=
+   |={⊤,∅}=>
+    ▷∃ s, "Hoc" ∷ own_channel ch cap s γ ∗
+     "Hcont" ∷
+    (match s with
+    (* Case: Sender is waiting, can complete immediately *)
+    | chan_rep.SndPending v =>
+          own_channel ch cap chan_rep.RcvCommit γ ={∅,⊤}=∗ Φ v true
+    (* Case: Channel is idle, need to wait for sender *)
+    | chan_rep.Idle =>
+          own_channel ch cap (chan_rep.RcvPending) γ ={∅,⊤}=∗
+              rcv_au_inner ch cap γ Φ
+    (* Case: Channel is closed *)
+    | chan_rep.Closed [] => own_channel ch cap s γ ={∅,⊤}=∗ Φ (default_val V) false
+    (* Case: Closed but still have values to drain *)
+    | chan_rep.Closed (v::rest) => (own_channel ch cap (chan_rep.Closed rest) γ ={∅,⊤}=∗ Φ v true)
+    (* Case: Buffered channel with values in buffer *)
+    | chan_rep.Buffered (v::rest) => (own_channel ch cap (chan_rep.Buffered rest) γ ={∅,⊤}=∗ Φ v true)
+    | _ => True
+    end).
+
+(** Fast path receive: immediate completion when possible *)
+Definition rcv_au_fast ch (cap: Z) (γ: chan_names) (Φ : V → bool → iProp Σ) : iProp Σ :=
+   |={⊤,∅}=>
+    ▷∃ s, "Hoc" ∷ own_channel ch cap s γ ∗
+     "Hcont" ∷
+    (match s with
+    (* Case: Sender is waiting, can complete immediately *)
+    | chan_rep.SndPending v =>
+          own_channel ch cap chan_rep.RcvCommit γ ={∅,⊤}=∗ Φ v true
+    (* Case: Channel is closed *)
+    | chan_rep.Closed [] => own_channel ch cap s γ ={∅,⊤}=∗ Φ (default_val V) false
+    (* Case: Channel is closed but still has values to drain *)
+    | chan_rep.Closed (v::rest) => (own_channel ch cap (chan_rep.Closed rest) γ ={∅,⊤}=∗ Φ v true)
+    (* Case: Buffered channel with values *)
+    | chan_rep.Buffered (v::rest) => (own_channel ch cap (chan_rep.Buffered rest) γ ={∅,⊤}=∗ Φ v true)
+    | _ => True
+    end).
+
+(** Inner atomic update for send completion (second phase of handshake) *)
+Definition send_au_inner ch (cap: Z) (γ: chan_names) (Φ : iProp Σ) : iProp Σ :=
+   |={⊤,∅}=>
+    ▷∃ s, "Hocinner" ∷ own_channel ch cap s γ ∗
+     "Hcontinner" ∷
+    (match s with
+    (* Case: Receiver has committed, complete the exchange *)
+    | chan_rep.RcvCommit =>
+           own_channel ch cap chan_rep.Idle γ ={∅,⊤}=∗ Φ
+    (* Case: Channel is closed, operation fails *)
+    | chan_rep.Closed draining => False
+    | _ => True
+    end).
+
+(** Slow path send: may need to block and wait *)
+Definition send_au_slow ch (cap: Z) (v : V) (γ: chan_names) (Φ : iProp Σ) : iProp Σ :=
+   |={⊤,∅}=>
+    ▷∃ s, "Hoc" ∷ own_channel ch cap s γ ∗
+     "Hcont" ∷
+    (match s with
+    (* Case: Receiver is waiting, can complete immediately *)
+    | chan_rep.RcvPending =>
+        own_channel ch cap (chan_rep.SndCommit v) γ ={∅,⊤}=∗ Φ
+    (* Case: Channel is idle, need to wait for receiver *)
+    | chan_rep.Idle =>
+          own_channel ch cap (chan_rep.SndPending v) γ ={∅,⊤}=∗
+              send_au_inner ch cap γ Φ
+    (* Case: Channel is closed, client must rule this out *)
+    | chan_rep.Closed draining => False
+    (* Case: Buffered channel with space available *)
+    | chan_rep.Buffered buff => 
+        if (length buff <? cap) 
+        then (own_channel ch cap (chan_rep.SndCommit v) γ ={∅,⊤}=∗ Φ)
+        else True
+    | _ => True
+    end).
+
+(** Fast path send: immediate completion when possible *)
+Definition send_au_fast ch (cap: Z) (v : V) (γ: chan_names) (Φ : iProp Σ) : iProp Σ :=
+   |={⊤,∅}=>
+    ▷∃ s, "Hoc" ∷ own_channel ch cap s γ ∗
+     "Hcont" ∷
+    (match s with
+    (* Case: Receiver is waiting, can complete immediately *)
+    | chan_rep.RcvPending =>
+        own_channel ch cap (chan_rep.SndCommit v) γ ={∅,⊤}=∗ Φ
+    (* Case: Channel is closed, client must rule this out *)
+    | chan_rep.Closed draining => False
+    (* Case: Buffered channel with space available *)
+    | chan_rep.Buffered buff => 
+        if (length buff <? cap) 
+        then (own_channel ch cap (chan_rep.SndCommit v) γ ={∅,⊤}=∗ Φ)
+        else True
+    | _ => True
+    end).
+
+(** Maps physical states to their logical representations with ghost state.
+    This is the key invariant that connects the physical implementation
+    to the logical specifications. *)
+Definition chan_logical (ch: loc) (cap: Z) (γ : chan_names) (s : chan_phys_state V): iProp Σ :=
+  match s with
+  | Idle =>
+       ∃ (Φr: V → bool → iProp Σ),
+           "Hoffer" ∷ offer_bundle_empty γ ∗
+           "Hpred" ∷ saved_pred_own γ.(offer_parked_pred_name) (DfracOwn 1) (K Φr) ∗
+            own_channel ch cap chan_rep.Idle γ
+
+  | SndWait v =>
+       ∃ (P: iProp Σ) (Φ: iProp Σ) (Φr: V → bool → iProp Σ),
+          "Hoffer" ∷ offer_bundle_half γ (Some (Snd v)) P Φ ∗
+          "HP" ∷ P ∗
+          "Hpred" ∷ saved_pred_own γ.(offer_parked_pred_name) (DfracOwn 1) (K Φr) ∗
+          "Hau" ∷ (P -∗ send_au_slow ch cap v γ Φ) ∗
+           own_channel ch cap chan_rep.Idle γ
+
+  | RcvWait =>
+       ∃ (P: iProp Σ) (Φr: V → bool → iProp Σ),
+         "Hoffer" ∷ offer_bundle_half γ (Some Rcv) P True ∗
+         "HP" ∷ P ∗
+         "Hpred" ∷ saved_pred_own γ.(offer_parked_pred_name) (DfracOwn (1/2)) (K Φr) ∗
+         "Hau" ∷ (P -∗ rcv_au_slow ch cap γ Φr) ∗
+         own_channel ch cap chan_rep.Idle γ
+
+  | SndDone v =>
+       ∃ (P: iProp Σ) (Φr: V → bool → iProp Σ),
+       "Hpred" ∷ saved_pred_own γ.(offer_parked_pred_name) (DfracOwn (1/2)) (K Φr) ∗
+       "Hoffer" ∷ offer_bundle_half γ (Some Rcv) P True ∗
+       "Hau" ∷ rcv_au_inner ch cap γ Φr ∗
+       own_channel ch cap (chan_rep.SndCommit v) γ
+
+  | RcvDone v =>
+       ∃ (P: iProp Σ) (Φ: iProp Σ) (Φr: V → bool → iProp Σ),
+         "Hoffer" ∷ offer_bundle_half γ (Some (Snd v)) P Φ ∗
+         "Hpred" ∷ saved_pred_own γ.(offer_parked_pred_name) (DfracOwn 1) (K Φr) ∗
+         "Hau" ∷ send_au_inner ch cap γ Φ ∗
+       own_channel ch cap chan_rep.RcvCommit γ
+
+  | Closed [] =>
+          own_channel ch cap (chan_rep.Closed []) γ ∗ 
+           "Hoffer" ∷ if (cap =? 0) then offer_bundle_empty γ else True
+
+  | Closed draining =>
+          own_channel ch cap (chan_rep.Closed draining) γ
+
+  | Buffered buff =>
+          own_channel ch cap (chan_rep.Buffered buff) γ
+  end.
+
+(** The main invariant protected by the channel's mutex.
+    This connects the physical heap state with the logical state. *)
+Definition chan_inv_inner (ch: loc) (cap: Z) (γ: chan_names) : iProp Σ :=
+  ∃ (s : chan_phys_state V),
+    "phys" ∷ chan_phys ch s ∗
+    "offer" ∷ chan_logical ch cap γ s.
+
+(** The public predicate that clients use to interact with channels.
+    This is persistent and provides access to the channel's capabilities. *)
+Definition is_channel (ch: loc) (cap: Z) (γ: chan_names) : iProp Σ :=
+  ∃ (mu_loc: loc),
+    "#cap" ∷ ch ↦s[(channel.Channel.ty t) :: "cap"]□ (W64 cap) ∗
+    "#mu" ∷ ch ↦s[(channel.Channel.ty t) :: "lock"]□ mu_loc ∗
+    "#lock" ∷ is_Mutex mu_loc (chan_inv_inner ch cap γ).
+
+Global Instance is_channel_pers ch cap γ : Persistent (is_channel cap ch γ).
+Proof.
+Admitted.
+
+Global Instance own_channel_timeless ch cap s γ : Timeless (own_channel ch cap s γ).
+Proof.
+Admitted.
+
+Lemma is_channel_not_null ch cap γ:
+  is_channel ch cap γ -∗ ⌜ch ≠ null⌝.
+Proof.
+Admitted.
+
 End base.
-
-
-
